label-free/Substitution.v
@@ -1,76 +1,319 @@
 Require Export Syntax.
+Require Import Metatheory.
 Require Import Arith.
 Require Import List.
 
 Open Scope label_free_is5_scope.
 
-Reserved Notation " {{ ctx1 // ctx2 }} Gamma " (at level 5).
+(* Term substitution *)
 
-Fixpoint subst_ctx (M0 : te_LF) (ctx1: ctx_LF) (ctx2: ctx_LF) :=
-match M0 with 
+(* We want to substitute M for nth hyp. in term N0, provided that the current context
+   is ctx. *)
+Fixpoint subst_t_outer (M0: te_LF) (n: nat) (ctx: ctx_LF) (N0: te_LF) (curr: ctx_LF) {struct N0} :=
+match N0 with
 | hyp_LF n => hyp_LF n
-| lam_LF A M =>lam_LF A {{ctx1 // ctx2}} M
-| appl_LF M N => appl_LF {{ctx1 // ctx2}}M {{ctx1 // ctx2}}N
+| lam_LF A M => lam_LF A (subst_t_outer M0 n ctx M curr)
+| appl_LF M N => appl_LF (subst_t_outer M0 n ctx M curr) (subst_t_outer M0 n ctx M curr)
 | box_LF M => 
-  match ctx1, ctx2 with
-    | bctx c1, bctx c2 => box_LF {{bctx (S c1) // bctx (S c2)}} M
-    | bctx c1, fctx c2 => box_LF {{bctx (S c1) // ctx2}} M
-    | fctx c1, bctx c2 => box_LF {{ctx1 // bctx (S c2)}} M
-    | fctx c1, fctx c2 => box_LF {{ctx1 // ctx2}} M
+  let w0 := var_gen (free_worlds_LF N0) in (* shouldn't we add sth? *)
+    box_LF (subst_t_outer M0 n ctx M (fctx w0))
+| unbox_LF M => unbox_LF (subst_t_outer M0 n ctx M curr)
+| unbox_fetch_LF w M => 
+  match (eq_ctx_LF_dec ctx w) with
+    | left _ => unbox_fetch_LF w (subst_t_inner M0 n M ctx) 
+    | right _ => unbox_fetch_LF w (subst_t_outer M0 n ctx M w)
   end
-| unbox_LF M => unbox_LF {{ctx1 // ctx2}} M
-| unbox_fetch_LF ctx M =>
-  let ctx' := if eq_ctx_LF_dec ctx ctx2 then ctx1 else ctx in
-  unbox_fetch_LF ctx' {{ctx1 // ctx2}} M
-| here_LF M => here_LF {{ctx1 // ctx2}} M
-| get_here_LF ctx M =>
-  let ctx' := if eq_ctx_LF_dec ctx ctx2 then ctx1 else ctx in
-  get_here_LF ctx' {{ctx1 // ctx2}}M
-| letdia_LF M N =>
-  match ctx1, ctx2 with
-    | bctx c1, bctx c2 => letdia_LF {{ctx1 // ctx2}}M {{bctx (S c1) // bctx (S c2)}}N
-    | bctx c1, fctx c2 => letdia_LF {{ctx1 // ctx2}}M {{bctx (S c1) // ctx2}}N
-    | fctx c1, bctx c2 => letdia_LF {{ctx1 // ctx2}}M {{ctx1 // bctx (S c2)}}N
-    | fctx c1, fctx c2 => letdia_LF {{ctx1 // ctx2}}M {{ctx1 // ctx2}}N
+| here_LF M => here_LF (subst_t_outer M0 n ctx M curr)
+| get_here_LF w M =>
+  match (eq_ctx_LF_dec ctx w) with
+    | left _ => get_here_LF w (subst_t_inner M0 n M ctx) 
+    | right _ => get_here_LF w (subst_t_outer M0 n ctx M w)
   end
-| letdia_get_LF ctx M N =>
-  let ctx' := if eq_ctx_LF_dec ctx ctx2 then ctx1 else ctx in
-  match ctx1, ctx2 with
-    | bctx c1, bctx c2 => letdia_get_LF ctx' {{ctx1 // ctx2}}M {{bctx (S c1) // bctx (S c2)}}N
-    | bctx c1, fctx c2 => letdia_get_LF ctx' {{ctx1 // ctx2}}M {{bctx (S c1) // ctx2}}N
-    | fctx c1, bctx c2 => letdia_get_LF ctx' {{ctx1 // ctx2}}M {{ctx1 // bctx (S c2)}}N
-    | fctx c1, fctx c2 => letdia_get_LF ctx' {{ctx1 // ctx2}}M {{ctx1 // ctx2}}N
+| letdia_LF M N => letdia_LF (subst_t_outer M0 n ctx M curr) (subst_t_outer M0 n ctx N curr)
+| letdia_get_LF w M N =>
+  match (eq_ctx_LF_dec ctx w) with
+    | left _ => letdia_get_LF w (subst_t_inner M0 n M ctx) (subst_t_outer M0 n ctx N w)
+    | right _ => letdia_get_LF w (subst_t_outer M0 n ctx M w) (subst_t_outer M0 n ctx N w)
   end
 end
-where " {{ c1 // c2 }} M " := (subst_ctx M c1 c2) : label_free_is5_scope.
+(* Current context is exactly the context in which we want to do susbtitution *)
+with subst_t_inner (M0: te_LF) (m: nat) (N0: te_LF) (curr: ctx_LF) {struct N0} :=
+match N0 with
+| hyp_LF n => if (eq_nat_dec n m) then M0 else hyp_LF n
+| lam_LF A M => lam_LF A (subst_t_inner M0 m M curr)
+| appl_LF M N => appl_LF (subst_t_inner M0 m M curr) (subst_t_inner M0 m N curr)
+| box_LF M =>
+  let w0 := var_gen (free_worlds_LF N0) in
+    box_LF (subst_t_outer M0 m curr M (fctx w0))
+| unbox_LF M => unbox_LF (subst_t_inner M0 m M curr)
+| unbox_fetch_LF w M =>
+  match (eq_ctx_LF_dec curr w) with
+    | left _ => unbox_fetch_LF w (subst_t_inner M0 m M curr) 
+    | right _ => unbox_fetch_LF w (subst_t_outer M0 m curr M w)
+  end
+| here_LF M => here_LF (subst_t_inner M0 m M curr)
+| get_here_LF w M =>
+  match (eq_ctx_LF_dec curr w) with
+    | left _ => get_here_LF w (subst_t_inner M0 m M curr) 
+    | right _ => get_here_LF w (subst_t_outer M0 m curr M w)
+  end
+| letdia_LF M N => letdia_LF (subst_t_inner M0 m M curr) (subst_t_inner M0 m N curr)
+| letdia_get_LF w M N =>
+  match (eq_ctx_LF_dec curr w) with
+    | left _ => letdia_get_LF w (subst_t_inner M0 m M curr) (subst_t_outer M0 m curr N w)
+    | right _ => letdia_get_LF w (subst_t_outer M0 m curr M w) (subst_t_outer M0 m curr N w)
+  end
+end.
 
-Definition open_ctx M c := subst_ctx M c (bctx 0). 
-Notation " M ^^ Gamma " := (open_ctx M Gamma) (at level 5) : label_free_is5_scope.
+Definition subst_t M n ctx N curr :=
+  if (eq_ctx_LF_dec ctx curr) then (subst_t_inner M n N curr) 
+  else (subst_t_outer M n ctx N curr). 
 
-(* TODO: this may be too little - we may need "outer" substitution with context switch 
-         and in that case when moving between contexts we will use "outer" substitution
-         to find the next occ. of "our" context *)
-Reserved Notation " [ M // n ] N " (at level 5).
+Notation " [ M // n | ctx ] [ N | curr ] " := 
+  (subst_t M n ctx N curr) (at level 5) : label_free_is5_scope.
 
-Fixpoint subst_LF (M: te_LF) (n: nat) (N: te_LF) : te_LF :=
-match N with
-| hyp_LF n' => if eq_nat_dec n n' then M else N
-| lam_LF A N' => lam_LF A [M//S n] N'
-| appl_LF N1 N2 => appl_LF ([M // n] N1) ([M // n] N2)
-| box_LF N' => box_LF ([M // n] N')
-| unbox_LF N' => unbox_LF ([M // n] N')
-| unbox_fetch_LF Ctx N' => N
-| here_LF N' => here_LF ([M // n] N')
-| get_here_LF Ctx N' => N
-| letdia_LF N1 N2 => letdia_LF ([M // n] N1) ([M // S n ] N2)
-| letdia_get_LF Ctx N1 N2 => N
-end
-where " [ M // n ] N " := (subst_LF M n N) : label_free_is5_scope.
-
-Fixpoint subst_list L n N :=
+Fixpoint subst_list L n N subst_ctx curr_ctx :=
 match L with
 | nil => N
-| M :: L' => [ M // n ] (subst_list L' (S n) N)
+| M :: L' => [M//n | subst_ctx] 
+             [subst_list L' (S n) N subst_ctx curr_ctx | curr_ctx]
 end.
+
+(* Context substitution *)
+
+Definition recalculate_ctx (ctx1: ctx_LF) (ctx2: ctx_LF) : prod ctx_LF ctx_LF :=
+   match ctx1, ctx2 with
+      | fctx w1', bctx w2' => (ctx1, bctx (S w2'))
+      | fctx w1', fctx w2' => (ctx1, ctx2)
+      | bctx w1', bctx w2' => (bctx (S w1'), bctx (S w2'))
+      | bctx w1', fctx w2' => (bctx (S w1'), ctx2)
+   end.
+
+(* We want to substitute ctx1 for every occ. of ctx2; our current context is curr.
+   We assume in subst_ctx_outer that curr <> ctx2 *)
+(* len_old is used to calculate shift in new hypotheses, when we substitute for some bctx
+   this should be set to 0 *)
+Fixpoint subst_ctx_outer (M0 : te_LF) (curr:ctx_LF) (ctx1: ctx_LF) (ctx2: ctx_LF) (len_old: nat) :=
+match M0 with 
+| hyp_LF n => hyp_LF n
+| lam_LF A M => lam_LF A (subst_ctx_outer M curr ctx1 ctx2 len_old)
+| appl_LF M N => appl_LF (subst_ctx_outer M curr ctx1 ctx2 len_old) 
+                         (subst_ctx_outer N curr ctx1 ctx2 len_old)
+| box_LF M => 
+  let w0 := var_gen (free_worlds_LF M) in
+  let (ctx1', ctx2') := recalculate_ctx ctx1 ctx2 in 
+    box_LF (subst_ctx_outer M (fctx w0) ctx1' ctx2' len_old)
+| unbox_LF M => unbox_LF (subst_ctx_outer M curr ctx1 ctx2 len_old)
+| unbox_fetch_LF w M =>
+  match (eq_ctx_LF_dec w ctx1) with
+  | left _ => unbox_fetch_LF w (subst_ctx_new M ctx1 ctx2 len_old)
+  | right _ => 
+    match (eq_ctx_LF_dec w ctx2) with
+      | left _ => unbox_fetch_LF w (subst_ctx_old M ctx1 ctx2 len_old)
+      | right _ => unbox_fetch_LF w (subst_ctx_outer M w ctx1 ctx2 len_old)
+    end
+   end
+| here_LF M => here_LF (subst_ctx_outer M curr ctx1 ctx2 len_old)
+| get_here_LF w M =>
+  match (eq_ctx_LF_dec w ctx1) with
+  | left _ => get_here_LF w (subst_ctx_new M ctx1 ctx2 len_old)
+  | right _ => 
+    match (eq_ctx_LF_dec w ctx2) with
+      | left _ => get_here_LF w (subst_ctx_old M ctx1 ctx2 len_old)
+      | right _ => get_here_LF w (subst_ctx_outer M w ctx1 ctx2 len_old)
+    end
+   end
+| letdia_LF M N =>
+  let (ctx1', ctx2') := recalculate_ctx ctx1 ctx2 in 
+    letdia_LF (subst_ctx_outer M curr ctx1 ctx2 len_old)
+              (subst_ctx_outer N curr ctx1' ctx2' len_old)
+| letdia_get_LF w M N =>
+  let (ctx1', ctx2') := recalculate_ctx ctx1 ctx2 in 
+  match (eq_ctx_LF_dec w ctx1) with
+  | left _ => letdia_get_LF w (subst_ctx_new M ctx1 ctx2 len_old) 
+                              (subst_ctx_outer N curr ctx1' ctx2' len_old)
+  | right _ => 
+    match (eq_ctx_LF_dec w ctx2) with
+      | left _ => letdia_get_LF w (subst_ctx_old M ctx1 ctx2 len_old) 
+                                  (subst_ctx_outer N curr ctx1' ctx2' len_old)
+      | right _ => letdia_get_LF w (subst_ctx_outer M w ctx1 ctx2 len_old) 
+                                   (subst_ctx_outer N curr ctx1' ctx2' len_old)
+    end
+   end
+end
+(* In subst_ctx_old we assume that current context is ctx2 *)
+with subst_ctx_old (M0 : te_LF) (ctx1: ctx_LF) (ctx2: ctx_LF) (len_old: nat) :=
+match M0 with 
+| hyp_LF n => hyp_LF n
+| lam_LF A M => lam_LF A (subst_ctx_old M ctx1 ctx2 (len_old))
+| appl_LF M N => appl_LF (subst_ctx_old M ctx1 ctx2 len_old) 
+                         (subst_ctx_old N ctx1 ctx2 len_old)
+| box_LF M =>
+  let w0 := var_gen (free_worlds_LF M) in
+  let (ctx1', ctx2') := recalculate_ctx ctx1 ctx2 in     
+    box_LF (subst_ctx_outer M (fctx w0) ctx1' ctx2' len_old)
+| unbox_LF M => unbox_LF (subst_ctx_old M ctx1 ctx2 len_old)
+| unbox_fetch_LF w M =>
+  match (eq_ctx_LF_dec w ctx1) with
+  | left _ => unbox_LF (subst_ctx_new M ctx1 ctx2 len_old)
+  | right _ => 
+    match (eq_ctx_LF_dec w ctx2) with
+      (* w = ctx2 will never really happen, since ctx2 is current context *) 
+      | left _ => unbox_fetch_LF w (subst_ctx_old M ctx1 ctx2 len_old)
+      | right _ => unbox_fetch_LF w (subst_ctx_outer M w ctx1 ctx2 len_old)
+    end
+   end
+| here_LF M => here_LF (subst_ctx_old M ctx1 ctx2 len_old)
+| get_here_LF w M =>
+  match (eq_ctx_LF_dec w ctx1) with
+  | left _ => here_LF (subst_ctx_new M ctx1 ctx2 len_old)
+  | right _ => 
+    match (eq_ctx_LF_dec w ctx2) with
+      | left _ => get_here_LF w (subst_ctx_old M ctx1 ctx2 len_old)
+      | right _ => get_here_LF w (subst_ctx_outer M w ctx1 ctx2 len_old)
+    end
+   end
+| letdia_LF M N => 
+  let (ctx1', ctx2') := recalculate_ctx ctx1 ctx2 in 
+    letdia_LF (subst_ctx_old M ctx1 ctx2 len_old) 
+              (subst_ctx_old N ctx1' ctx2' len_old)
+| letdia_get_LF w M N =>
+  let (ctx1', ctx2') := recalculate_ctx ctx1 ctx2 in 
+  match (eq_ctx_LF_dec w ctx1) with
+  | left _ => letdia_LF (subst_ctx_new M ctx1 ctx2 len_old) (subst_ctx_old M ctx1' ctx2' len_old)
+  | right _ => 
+    match (eq_ctx_LF_dec w ctx2) with
+      | left _ => letdia_get_LF w (subst_ctx_old M ctx1 ctx2 len_old) (subst_ctx_old M ctx1' ctx2' len_old) 
+      | right _ => letdia_get_LF w (subst_ctx_outer M w ctx1 ctx2 len_old) (subst_ctx_old M ctx1' ctx2' len_old) 
+    end
+  end
+end
+(* In subst_ctx_new we assume that current context is ctx1 *)
+with subst_ctx_new (M0 : te_LF) (ctx1: ctx_LF) (ctx2: ctx_LF) (len_old: nat) :=
+match M0 with 
+| hyp_LF n => hyp_LF (len_old+n)
+| lam_LF A M => lam_LF A (subst_ctx_new M ctx1 ctx2 len_old)
+| appl_LF M N => appl_LF (subst_ctx_new M ctx1 ctx2 len_old) 
+                         (subst_ctx_new N ctx1 ctx2 len_old)
+| box_LF M =>
+  let w0 := var_gen (free_worlds_LF M) in
+  let (ctx1', ctx2') := recalculate_ctx ctx1 ctx2 in 
+    box_LF (subst_ctx_outer M (fctx w0) ctx1' ctx2' len_old)
+| unbox_LF M => unbox_LF (subst_ctx_new M ctx1 ctx2 len_old)
+| unbox_fetch_LF w M =>
+  match (eq_ctx_LF_dec w ctx1) with
+  (* w = ctx1 will never really happen, since ctx1 is current context *) 
+  | left _ => unbox_fetch_LF w (subst_ctx_new M ctx1 ctx2 len_old)
+  | right _ => 
+    match (eq_ctx_LF_dec w ctx2) with
+      | left _ => unbox_LF (subst_ctx_old M ctx1 ctx2 len_old)
+      | right _ => unbox_fetch_LF w (subst_ctx_outer M w ctx1 ctx2 len_old)
+    end
+   end
+| here_LF M => here_LF (subst_ctx_new M ctx1 ctx2 len_old)
+| get_here_LF w M =>
+  match (eq_ctx_LF_dec w ctx1) with
+  | left _ => get_here_LF w (subst_ctx_new M ctx1 ctx2 len_old)
+  | right _ => 
+    match (eq_ctx_LF_dec w ctx2) with
+      | left _ => here_LF (subst_ctx_old M ctx1 ctx2 len_old)
+      | right _ => get_here_LF w (subst_ctx_outer M w ctx1 ctx2 len_old)
+    end
+   end
+| letdia_LF M N => 
+  let (ctx1', ctx2') := recalculate_ctx ctx1 ctx2 in 
+    letdia_LF (subst_ctx_new M ctx1 ctx2 len_old) 
+              (subst_ctx_new N ctx1' ctx2' len_old)
+| letdia_get_LF w M N =>
+  let (ctx1', ctx2') := recalculate_ctx ctx1 ctx2 in 
+  match (eq_ctx_LF_dec w ctx1) with
+  | left _ => letdia_get_LF w (subst_ctx_new M ctx1 ctx2 len_old) (subst_ctx_old M ctx1' ctx2' len_old)
+  | right _ => 
+    match (eq_ctx_LF_dec w ctx2) with
+      | left _ => letdia_LF (subst_ctx_old M ctx1 ctx2 len_old) (subst_ctx_old M ctx1' ctx2' len_old) 
+      | right _ => letdia_get_LF w (subst_ctx_outer M w ctx1 ctx2 len_old) (subst_ctx_old M ctx1' ctx2' len_old) 
+    end
+  end
+end.
+
+Definition subst_ctx M c1 c2 curr len_old :=
+match (eq_ctx_LF_dec c1 c2) with
+| left _ => M
+| right _ => 
+  if (eq_ctx_LF_dec curr c1) then subst_ctx_new M c1 c2 len_old
+  else if (eq_ctx_LF_dec curr c2) then subst_ctx_old M c1 c2 len_old
+       else subst_ctx_outer M curr c1 c2 len_old
+end.
+
+Notation " {{ c1 // c2 }} [ M | curr , m ] " := 
+  (subst_ctx M c1 c2 curr m) (at level 5) : label_free_is5_scope.
+
+Definition open_ctx M ctx curr := subst_ctx M ctx (bctx 0) curr 0.
+
+Notation " M ^^ [ w | w' ] " := (open_ctx M w w') (at level 10) : label_free_is5_scope.
+
+Section Lemmas.
+
+Lemma no_unbound_worlds_subst_w_id:
+forall M w k w'
+  (H_unbound: unbound_worlds k M = nil),
+  {{w//bctx k}}[M | w', 0] = M.
+Admitted.
+
+Lemma closed_w_subst_id:
+forall M w n w'
+  (HT: lc_w_n_LF M n),
+  {{w//bctx n}} [M | w', 0] = M.
+intros;
+apply no_unbound_worlds_subst_w_id;
+apply closed_no_unbound_worlds;
+assumption.
+Qed.
+
+Lemma subst_order_irrelevant:
+forall N M n m w w' w''
+  (H_LC: lc_w_LF M),
+  subst_ctx ([M//n | w''] [N | w']) w (bctx m) w' 0 = 
+  [M//n | w''] [(subst_ctx N w (bctx m) w' 0) | w'].
+Admitted.
+
+Lemma subst_w_comm:
+forall M w w' w'' n w0 w1 k
+  (Neq: w'' <> w),
+  {{fctx w'//fctx w''}}[({{fctx w//bctx n}}[M | w0, 0]) | w1, k] = {{fctx w//bctx n}}[({{fctx w'//fctx w''}}[M | w1, k]) | w0, 0].
+Admitted.
+
+Lemma subst_id:
+forall M w n w0 k w0'
+  (HT: fresh_world_LF w M),
+  {{bctx n//fctx w}}[({{fctx w//bctx n}}[M | w0, 0]) | w0', k] = M.
+Admitted.
+
+(* This is just one option of neutral substitution! *)
+Lemma subst_neutral:
+forall M w w' n  k
+  (HT: lc_w_n_LF M n),
+  {{fctx w//bctx n}}[({{bctx n//fctx w'}}[M | fctx w', k]) | fctx w, 0] = {{fctx w//fctx w'}}[ M | fctx w', k].
+Admitted.
+
+Lemma subst_neutral':
+forall M w w' n  k
+  (HT: lc_w_n_LF M n),
+  {{fctx w//bctx n}}[({{bctx n//fctx w'}}[M | fctx w, k]) | fctx w, 0] = {{fctx w//fctx w'}}[ M | fctx w, k].
+Admitted.
+
+Lemma subst_neutral'':
+forall M w w' w0 n  k
+  (HT: lc_w_n_LF M n),
+  {{fctx w//bctx n}}[({{bctx n//fctx w'}}[M | fctx w0, k]) | fctx w0, 0] = {{fctx w//fctx w'}}[ M | fctx w0, k].
+Admitted.
+
+Lemma closed_step_opening:
+forall M n w w0
+  (HT: lc_w_n_LF M (S n)),
+  lc_w_n_LF ({{fctx w//bctx n}}[M | w0, 0]) n.
+Admitted.
+
+End Lemmas.
 
 Close Scope label_free_is5_scope.
